\documentclass[fleqn]{article}

\usepackage[scale=0.75, twoside, bindingoffset=5mm]{geometry}
\usepackage[onehalfspacing]{setspace}

\usepackage{kotex}
\usepackage{amsmath}
\usepackage{enumerate}


\begin{document}

\begin{enumerate}

	\item Discrete Distributions
	
	\begin{enumerate}
	
		\item binomial distribution
		\begin{displaymath}
			p(y) = \binom{n}{y} p^{y} (1-p)^{n-y} \quad ; 
			\quad y=0,1,\cdots, n
		\end{displaymath}
		
		
		\item geometric distribution
		\begin{displaymath}
			p(y) = p(1-p)^{y-1} \quad ; 
			\quad y=1, 2, \cdots
		\end{displaymath}
		
		
		\item hypergeometric distribution
		\begin{displaymath}
			p(y) = \frac{ \binom{r}{y} \binom{N-r}{n-y} }
			{\binom{N}{n}} \quad ; \quad
			y = 0, 1, \cdots, n \ if \ n \le r, 
			\ y = 0, 1, \cdots, r \ if \ n > r
		\end{displaymath}
		
				
		\item poisson distribution
		\begin{displaymath}
			p(y) = \frac{\lambda^{y} e^{-\lambda}}{y!} \quad ;
			\quad y = 0, 1, 2, \cdots
		\end{displaymath}
		
		
		\item negative binomial distribution
		\begin{displaymath}
			p(y) = \binom{y-1}{r-1} p^{y} (1-p)^{y-r} \quad ;
			\quad y = r, r+1, \cdots
		\end{displaymath}	

	\end{enumerate}


	\item Continuous Distributions
	
	\begin{enumerate}		
		
		\item uniform distribution
		\begin{displaymath}
			f(y) = \frac{1}{\theta_{2} - \theta_{1}} \quad ;
			\quad \theta_{1} \le y \le \theta_{2}
		\end{displaymath}	
		
		\item normal distribution
		\begin{displaymath}
			f(y) = \frac{1}{\sigma \sqrt{2\pi}}
			\exp \left[ - \left( \frac{1}{2\sigma^{2}} \right) 
			(y-\mu)^{2} \right] \quad ; 
			\quad -\infty < y < \infty
		\end{displaymath}
		
		\item exponential distribution
		\begin{displaymath}
			f(y) = \frac{1}{\beta} e^{-y/\beta}, \beta>0 \quad ;
			\quad 0 \le y < \infty
		\end{displaymath}
		
		
		\item gamma distribution
		\begin{displaymath}
			f(y) = \left[ \frac{1}{\Gamma(\alpha) \beta^{\alpha}} \right]
			y^{\alpha - 1} e^{-y/\beta} \quad ;
			\quad 0 < y < \infty
		\end{displaymath}
		
		
		\item chi-square distribution
		\begin{displaymath}
			f(\chi^{2}) = 
			\frac{(\chi^2)^{(\nu/2)-1} e^{-\chi^{2}/2}}
			{2^{\nu/2} \Gamma (\nu/2) } \quad ;
			\quad \chi^{2} > 0
		\end{displaymath}
		
		\item beta distribution
		\begin{displaymath}
			f(y) = \left[ 
			\frac{\Gamma(\alpha + \beta)}{\Gamma(\alpha) \Gamma(\beta)} 
			\right]
			y^{\alpha - 1} (1-y)^{\beta - 1} \quad ;
			\quad 0 < y < 1
		\end{displaymath}
		
	\end{enumerate}	
	
	
\end{enumerate}

\end{document}